examples/BirthdayBook.thy
@@ -12,7 +12,7 @@ consts
 zstore BirthdayBook = 
   known :: "\<bbbP> name"
   birthday :: "name \<Zpfun> date"
-  where "known = dom birthday"
+  where "known = dom birthday" "known \<subseteq> NAME" "ran(birthday) \<subseteq> DATE"
 
 zoperation AddBirthday = 
   over BirthdayBook
@@ -20,7 +20,7 @@ zoperation AddBirthday =
   pre "name \<notin> known"
   update "[known \<leadsto> known \<union> {name}, birthday \<leadsto> birthday \<oplus> {name \<mapsto> date}]"
 
-lemma "H{BirthdayBook_inv} AddBirthday (n, d) {BirthdayBook_inv}"
+lemma AddBirthday_inv: "AddBirthday (n, d) preserves BirthdayBook_inv"
   by zpog_full
 
 zoperation FindBirthday =
@@ -29,18 +29,26 @@ zoperation FindBirthday =
   pre "name \<in> dom birthday"
   where "date = birthday(name)"
 
-lemma "H{BirthdayBook_inv} FindBirthday (n, d) {BirthdayBook_inv}"
+lemma FindBirthday_inv: "FindBirthday (n, d) preserves BirthdayBook_inv"
   by zpog_full
 
 zoperation Remind =
   over BirthdayBook
-  params today\<in>DATE cards\<in>"\<bbbP> DATE"
+  params today\<in>DATE cards\<in>"\<bbbP> NAME"
   where "cards = {n \<in> known. birthday(n) = today}"
+
+lemma Remind_inv: "Remind (n, d) preserves BirthdayBook_inv"
+  by zpog_full
 
 zmachine BirthdayBookSys = 
   init "[known \<leadsto> {}, birthday \<leadsto> {\<mapsto>}]"
   operations AddBirthday FindBirthday Remind
 
+definition [z_defs]: "BirthdayBook_axioms = (NAME \<noteq> {} \<and> DATE \<noteq> {})"
+
+lemma BirthdayBook_deadlock_free: "BirthdayBook_axioms \<Longrightarrow> deadlock_free BirthdayBookSys"
+  unfolding BirthdayBookSys_def
+  by (deadlock_free "BirthdayBook_inv :: BirthdayBook \<Rightarrow> bool" invs: AddBirthday_inv FindBirthday_inv Remind_inv) 
 
 def_consts NAME = "{STR ''Simon''}" 
 def_consts DATE = "{STR ''25/08/1983''}"
